x86/TablesEncodeproof.v
@@ -7,25 +7,35 @@ Require Import SymbtableEncode SymbtableDecode.
 Require Import ShstrtableEncode ShstrtableDecode.
 Require Import ReloctablesEncode ReloctablesDecode.
 Require Import RelocProgSemantics2 RelocProgSemantics3.
+Require Import TablesEncode.
 
 Import ListNotations.
+
+Definition match_prog (p tp:RelocProgram.program) :=
+  transf_program p = OK tp.
+
+Lemma transf_program_match:
+  forall p tp, transf_program p = OK tp -> match_prog p tp.
+Proof.
+  intros. red. auto.
+Qed.
+
 (** Preservation of semantics under permutation *)
 Section PRESERVATION.
 
 Context `{external_calls_prf: ExternalCalls}.
 
-Variables prog prog1 prog2 prog3 tprog: RelocProgram.program.
+Variables prog tprog: RelocProgram.program.
 
-Hypothesis transf_str_encode: StrtableEncode.transf_program prog = OK prog1.
-Hypothesis transf_symb_encode: SymbtableEncode.transf_program prog1 = OK prog2.
-Hypothesis transf_reloc_encode: ReloctablesEncode.transf_program prog2 = OK prog3.
-Hypothesis transf_shstr_encode: ShstrtableEncode.transf_program prog3 = OK tprog.
+Hypothesis transf_encode: TablesEncode.transf_program prog = OK tprog.
 
 Hypothesis valid_reloctables:
   forall id, Forall valid_relocentry (get_reloctable id (prog_reloctables prog)).
 
 Hypothesis valid_symbentries_p:
-  Forall (valid_symbentry (RelocProgram.prog_strtable prog1)) (RelocProgram.prog_symbtable prog1).
+  forall strmap sbytes,
+    get_strings_map_bytes (fold_right acc_symbols nil (prog_symbtable prog)) = OK (strmap, sbytes) ->
+    Forall (valid_symbentry strmap) (RelocProgram.prog_symbtable prog).
 
 Hypothesis empty_strtable:
   prog_strtable prog = Maps.PTree.empty Z.
@@ -48,141 +58,124 @@ Hypothesis prog_strings_eq:
 Hypothesis prog_strings_not_empty:
   Forall (fun '(_, lb) => lb <> []) prog_strings.
 
-Lemma strtable_encode_spec:
-  forall prog prog1,
-    StrtableEncode.transf_program prog = OK prog1 ->
-    prog_defs prog = prog_defs prog1 /\
-    prog_public prog = prog_public prog1 /\
-    prog_main prog = prog_main prog1 /\
-    prog_symbtable prog = prog_symbtable prog1 /\
-    prog_reloctables prog = prog_reloctables prog1 /\
-    prog_senv prog = prog_senv prog1 /\
-    (exists strmap sbytes,
-      get_strings_map_bytes (fold_right acc_symbols nil (prog_symbtable prog)) = OK (strmap, sbytes) /\
-      prog_strtable prog1 = strmap /\
-      prog_sectable prog1 = prog_sectable prog ++ create_strtab_section sbytes :: nil
-    ).
+
+Lemma acc_symbols_in_in_symbols:
+  forall s x0 l,
+    fold_right acc_symbol_strings (OK l) (fold_right acc_symbols [] s) = OK x0 ->
+    forall i,
+      In i (map fst x0) ->
+      In i (map fst l) \/ exists a, In a s /\ symbentry_id a = Some i.
 Proof.
-  clear.
-  unfold StrtableEncode.transf_program. intros prog prog1 TF.
-  monadInv TF. repeat destr_in EQ0. simpl; auto.
-  repeat split.
-  rewrite EQ. eauto.
+  induction s; simpl; intros x0 l FOLD i IN.
+  - inv FOLD. auto.
+  - unfold acc_symbols at 1 in FOLD.
+    destr_in FOLD; eauto.
+    + simpl in FOLD.
+      unfold acc_symbol_strings at 1 in FOLD. monadInv FOLD.
+      repeat destr_in EQ0.
+      simpl in IN. destruct IN as [eq | IN]; subst.
+      right; eexists; split; eauto.
+      exploit IHs. eauto. eauto. intros [A | [a0 [INs EQs]]]; eauto.
+    + exploit IHs; eauto. intros [A | [a0 [INs EQs]]]; eauto.
 Qed.
 
-Lemma symbtable_encode_spec:
-  forall prog prog1,
-    SymbtableEncode.transf_program prog = OK prog1 ->
-    prog_defs prog = prog_defs prog1 /\
-    prog_public prog = prog_public prog1 /\
-    prog_main prog = prog_main prog1 /\
-    prog_symbtable prog = prog_symbtable prog1 /\
-    prog_strtable prog = prog_strtable prog1 /\
-    prog_reloctables prog = prog_reloctables prog1 /\
-    prog_senv prog = prog_senv prog1 /\
-    (exists s,
-        create_symbtable_section (prog_strtable prog) (prog_symbtable prog) = OK s /\
-        prog_sectable prog1 = prog_sectable prog ++ s :: nil
-    ).
+Lemma gsmb_valid_strtable:
+  forall pi strmap sbytes,
+         let symbols := fold_right acc_symbols [] (prog_symbtable pi) in
+         get_strings_map_bytes symbols = OK (strmap, sbytes) ->
+         forall
+         x (EQ0 : fold_right acc_symbol_strings (OK []) (fold_right acc_symbols [] (prog_symbtable pi)) = OK x)
+         (LNR: list_norepet (filter (fun o => match o with None => false | _ => true end)
+                                    (map symbentry_id (prog_symbtable pi))))
+,
+    valid_strtable x strmap.
 Proof.
-  clear.
-  unfold SymbtableEncode.transf_program. intros prog prog1 TF.
-  monadInv TF. repeat destr_in EQ0. simpl; auto.
-  repeat split.
-  rewrite EQ. eauto.
+  intros pi strmap sbytes symbols GSMB x EQ0 LNR.
+  unfold valid_strtable.
+
+  assert (LNR': list_norepet (map fst x)).
+  {
+    revert x EQ0 LNR.
+    generalize (prog_symbtable pi). clear.
+    induction s; simpl; intros; eauto.
+    - inv EQ0. constructor.
+    - unfold acc_symbols at 1 in EQ0.
+      destr_in EQ0; eauto. simpl in EQ0.
+      unfold acc_symbol_strings at 1 in EQ0. monadInv EQ0.
+      exploit IHs. apply EQ. inv LNR; auto.
+      repeat destr_in EQ1. simpl. intros; constructor; auto.
+      intro INi.
+      eapply acc_symbols_in_in_symbols in INi; eauto. simpl in INi. destruct INi as [[]|(aa & IN & EQa)].
+      inv LNR. apply H2.
+      apply filter_In. split; auto.
+      rewrite in_map_iff. eexists; split; eauto.
+  }
+  unfold get_strings_map_bytes in GSMB.
+  unfold symbols in GSMB. rewrite EQ0 in GSMB. simpl in GSMB. repeat destr_in GSMB.
+  exists z; split; auto.
+  revert z Heqp l.
+  assert (valid_strtable_thr x (Maps.PTree.empty Z) 1 /\ 0 < 1).
+  {
+    split.
+    constructor; setoid_rewrite Maps.PTree.gempty; congruence.
+    omega.
+  }
+  generalize strmap.
+  destruct H as (VALID & POS).
+  revert VALID POS.
+  generalize (Maps.PTree.empty Z) 1.
+  clear -LNR'.
+  assert (forall elt, In elt x -> In elt x) by auto. revert H.
+  generalize x at 1 4.
+  induction x0; simpl.
+  - intros; eauto. inv Heqp. auto.
+  - intros IN t z VALID POS t0 z1 FOLD LT.
+    destr_in FOLD.
+    eapply IHx0 in FOLD. auto. eauto.
+    constructor; repeat setoid_rewrite Maps.PTree.gsspec.
+    + intros i0 j x1 y bytesx bytesy ox oy. repeat destr.
+      * intros Tx Ty Bx By Diff Ox Oy. inv Tx. inv VALID.
+        specialize (thr _ _ _ _ Ty By Oy). omega.
+      * intros Tx Ty Bx By Diff Ox Oy. inv Ty. inv VALID.
+        specialize (thr _ _ _ _ Tx Bx Ox). omega.
+      * inv VALID; eauto.
+    + intros i0 x1 bytesx ox Tx Bx Ox. destr_in Tx.
+      * inv Tx. erewrite Assoc.in_lnr_get_assoc in Bx. 3: apply IN; left; reflexivity. inv Bx; omega.
+        auto.
+      * inv VALID.
+        eapply thr in Bx; eauto. omega.
+    + intros i0 x1 EQ. destr_in EQ.
+      * inv EQ. erewrite Assoc.in_lnr_get_assoc; eauto.
+      * inv VALID; eauto.
+    + intros i0 x1 EQ. destr_in EQ.
+      * inv EQ.
+        apply acc_strmap_fold_lt in FOLD. change (two_p 32) with (Int.max_unsigned + 1).
+        omega.
+      * inv VALID; eauto.
+    + intros i0 EQ. destr_in EQ. inv EQ.
+      omega. inv VALID; eauto.
+    + omega.
+    + auto.
 Qed.
 
-Lemma reloctables_encode_spec:
-  forall prog prog1,
-    ReloctablesEncode.transf_program prog = OK prog1 ->
-    prog_defs prog = prog_defs prog1 /\
-    prog_public prog = prog_public prog1 /\
-    prog_main prog = prog_main prog1 /\
-    prog_symbtable prog = prog_symbtable prog1 /\
-    prog_strtable prog = prog_strtable prog1 /\
-    prog_reloctables prog = prog_reloctables prog1 /\
-    prog_senv prog = prog_senv prog1 /\
-    prog_sectable prog1 = prog_sectable prog ++ create_reloctables_sections prog.
+Lemma valid_strtable_p:
+  forall strmap sbytes,
+    get_strings_map_bytes (fold_right acc_symbols nil (prog_symbtable prog)) = OK (strmap, sbytes) ->
+    valid_strtable prog_strings strmap.
 Proof.
-  clear.
-  unfold ReloctablesEncode.transf_program. intros prog prog1 TF.
-  repeat destr_in TF. simpl; auto.
-  repeat split.
+  intros. eapply gsmb_valid_strtable; eauto.
 Qed.
-
-Lemma shstrtable_encode_spec:
-  forall prog prog1,
-    ShstrtableEncode.transf_program prog = OK prog1 ->
-    prog_defs prog = prog_defs prog1 /\
-    prog_public prog = prog_public prog1 /\
-    prog_main prog = prog_main prog1 /\
-    prog_symbtable prog = prog_symbtable prog1 /\
-    prog_strtable prog = prog_strtable prog1 /\
-    prog_reloctables prog = prog_reloctables prog1 /\
-    prog_senv prog = prog_senv prog1 /\
-    prog_sectable prog1 = prog_sectable prog ++ create_shstrtab_section :: nil.
-Proof.
-  clear.
-  unfold ShstrtableEncode.transf_program. intros prog prog1 TF.
-  repeat destr_in TF. simpl; auto.
-  repeat split.
-Qed.
-
-
-Lemma valid_strtable_p: valid_strtable prog_strings (RelocProgram.prog_strtable prog1).
-Proof.
-  generalize transf_str_encode. unfold StrtableEncode.transf_program. intro H. monadInv H.
-  repeat destr_in EQ0. simpl in *.
-  unfold get_strings_map_bytes in EQ. rewrite prog_strings_eq in EQ. simpl in EQ. repeat destr_in EQ.
-  exploit StrtableEncode.transf_program_valid_strtable. eauto. eauto. eauto. simpl. auto.
-Qed.
-
-
-Lemma genv_senv_add_external_global:
-  forall exts ge a,
-    RelocProgSemantics.Genv.genv_senv (RelocProgSemantics.add_external_global exts ge a) =
-    RelocProgSemantics.Genv.genv_senv ge.
-Proof.
-  unfold RelocProgSemantics.add_external_global. intros.
-  destr.
-Qed.
-
-Lemma genv_senv_add_external_globals:
-  forall st exts ge,
-    RelocProgSemantics.Genv.genv_senv (RelocProgSemantics.add_external_globals exts ge st) =
-    RelocProgSemantics.Genv.genv_senv ge.
-Proof.
-  induction st; simpl; intros; eauto.
-  rewrite IHst.
-  apply genv_senv_add_external_global.
-Qed.
-
-Lemma genv_senv_same:
-  RelocProgSemantics1.genv_senv (RelocProgSemantics1.globalenv tprog) =
-  RelocProgSemantics1.genv_senv (RelocProgSemantics1.globalenv prog).
-Proof.
-  unfold RelocProgSemantics1.globalenv. simpl.
-  unfold RelocProgSemantics1.genv_senv. simpl.
-  unfold RelocProgSemantics.globalenv.
-  rewrite ! genv_senv_add_external_globals. simpl.
-  exploit strtable_encode_spec; eauto. exploit symbtable_encode_spec; eauto.
-  exploit reloctables_encode_spec; eauto. exploit shstrtable_encode_spec; eauto.
-  intuition congruence.
-Qed.
-
 
 Lemma tables_encode_spec:
-  forall prog prog1 prog2 prog3 tprog,
-    StrtableEncode.transf_program prog = OK prog1 ->
-    SymbtableEncode.transf_program prog1 = OK prog2 ->
-    ReloctablesEncode.transf_program prog2 = OK prog3 ->
-    ShstrtableEncode.transf_program prog3 = OK tprog ->
+  forall prog tprog,
+    TablesEncode.transf_program prog = OK tprog ->
     prog_defs prog = prog_defs tprog /\
     prog_public prog = prog_public tprog /\
     prog_main prog = prog_main tprog /\
     prog_symbtable prog = prog_symbtable tprog /\
     prog_reloctables prog = prog_reloctables tprog /\
     prog_senv prog = prog_senv tprog /\
+    length (prog_sectable prog) = 3%nat /\
     exists (strmap : Maps.PTree.t Z) (sbytes : list byte) symt,
       get_strings_map_bytes (fold_right acc_symbols nil (prog_symbtable prog)) =
       OK (strmap, sbytes) /\
@@ -197,16 +190,27 @@ Lemma tables_encode_spec:
                        create_shstrtab_section].
 Proof.
   clear. intros.
-  exploit strtable_encode_spec; eauto.
-  exploit symbtable_encode_spec; eauto.
-  exploit reloctables_encode_spec; eauto.
-  exploit shstrtable_encode_spec; eauto. intuition try congruence.
-  destruct H31 as (strmap & sbytes & GSM & STR & SEC).
-  destruct H34 as (symt & CSS & EQ).
-  exists strmap, sbytes, symt; intuition try congruence.
-  rewrite H32, H33, EQ, SEC. simpl.
-  rewrite <- app_assoc. simpl.
-  rewrite <- ! app_assoc. simpl.
+  unfold transf_program in H.
+  monadInv H.
+  repeat destr_in EQ0.
+  monadInv H0.
+  repeat destr_in EQ1. simpl. repeat split; auto.
+  {
+    apply beq_nat_true in Heqb. rewrite app_length in Heqb.
+    simpl in Heqb. omega.
+  }
+  rewrite EQ. exists t, l, x. auto.
+Qed.
+
+Lemma genv_senv_same:
+  RelocProgSemantics1.genv_senv (RelocProgSemantics1.globalenv tprog) =
+  RelocProgSemantics1.genv_senv (RelocProgSemantics1.globalenv prog).
+Proof.
+  unfold RelocProgSemantics1.globalenv. simpl.
+  unfold RelocProgSemantics1.genv_senv. simpl.
+  unfold RelocProgSemantics.globalenv.
+  rewrite ! RelocProgSemantics.genv_senv_add_external_globals. simpl.
+  exploit tables_encode_spec; eauto.
   intuition congruence.
 Qed.
 
@@ -217,20 +221,16 @@ Proof.
   unfold RelocProgSemantics1.globalenv. simpl.
   unfold RelocProgSemantics.globalenv.
   exploit tables_encode_spec; eauto.
-  intros (EQdefs & EQpublic & EQmain & EQsymt & EQreloct & EQsenv & strmap & sbytes & symt
+  intros (EQdefs & EQpublic & EQmain & EQsymt & EQreloct & EQsenv & LEN & strmap & sbytes & symt
           & GSMB & CSS & EQstrt & EQsect).
   f_equal; try intuition congruence.
   f_equal; try intuition congruence.
   rewrite EQsect.
-  cut (length (prog_sectable prog) = 3%nat). intro LEN.
+  f_equal. unfold SeqTable.SeqTable.get. unfold sec_code_id.
   destruct (prog_sectable prog) eqn:?; simpl in LEN; try congruence.
   destruct s0 eqn:?; simpl in LEN; try congruence.
-  destruct l eqn:?; simpl in LEN; try congruence.
-  destruct l0 eqn:?; simpl in LEN; try congruence. simpl. auto.
-  unfold StrtableEncode.transf_program in transf_str_encode.
-  monadInv transf_str_encode. repeat destr_in EQ0. simpl in *.
-  apply beq_nat_true in Heqb. rewrite app_length in Heqb.
-  simpl in Heqb. omega.
+  destruct l eqn:?; simpl in LEN; try congruence. simpl.
+  destruct l0 eqn:?; simpl in LEN; try congruence.
 Qed.
 
 Lemma genv_reloc_same:
@@ -254,47 +254,37 @@ Proof.
   apply genv_genv_same.
 Qed.
 
+Lemma decode_tables_correct:
+  decode_tables tprog = OK prog.
+Proof.
+  exploit tables_encode_spec; eauto.
+  intros (EQdefs & EQpublic & EQmain & EQsymt & EQreloct & EQsenv & LEN & strmap & sbytes & symt
+          & GSMB & CSS & EQstrt & EQsect).
+  unfold decode_tables.
+  rewrite EQsect.
+  destruct (prog_sectable prog) eqn:?; simpl in LEN; try omega.
+  destruct s0 eqn:?; simpl in LEN; try omega.
+  destruct l eqn:?; simpl in LEN; try omega.
+  destruct l0 eqn:?; simpl in LEN; try omega. simpl.
+  rewrite decode_encode_reloctable. simpl.
+  rewrite decode_encode_reloctable. simpl.
+  erewrite decode_string_map_correct'. 2: eauto. simpl.
+  rewrite GSMB. simpl.
+  erewrite decode_create_symtable_section. 5: eauto. simpl.
+  destruct prog; simpl in *. subst. f_equal. f_equal; intuition try congruence.
+  destruct tprog; simpl. destruct prog_reloctables; simpl; auto.
+  all: eauto.
+  eapply valid_strtable_p; eauto.
+  apply valid_reloctables with (id := RELOC_CODE).
+  apply valid_reloctables with (id := RELOC_DATA).
+Qed.
+
 Theorem transf_program_correct rs:
   forward_simulation (RelocProgSemantics2.semantics prog rs)
                      (RelocProgSemantics3.semantics tprog rs).
 Proof.
-  generalize(ShstrtableDecode.transf_program_inv_correct _ transf_shstr_encode). intro shstr_decode.
-  generalize (fun v1 v2 => ReloctablesDecode.transf_program_inv_correct
-                _ v1 v2 transf_reloc_encode).
-  replace (prog_reloctables prog2) with (prog_reloctables prog).
-  intro reloc_decode.
-  trim reloc_decode. apply valid_reloctables with (id := RELOC_CODE).
-  trim reloc_decode. apply valid_reloctables with (id := RELOC_DATA).
-  Focus 2.
-  exploit strtable_encode_spec; eauto. exploit symbtable_encode_spec; eauto. intuition congruence.
-  exploit SymbtableDecode.transf_program_inv_correct. 3: apply valid_strtable_p.
-  all: eauto.
-  replace (prog_symbtable prog1) with (prog_symbtable prog). auto.
-  {
-    exploit strtable_encode_spec. eauto. intuition congruence.
-  }
-  intro symb_decode.
-  generalize (StrtableDecode.transf_program_inv_correct _ empty_strtable transf_str_encode). intro str_decode.
-  eapply forward_simulation_step with (match_states := fun (e1 e2: Asm.state) => e1 = e2).
-  - simpl. intro id. f_equal.
-    unfold RelocProgSemantics1.globalenv. simpl.
-    unfold RelocProgSemantics1.genv_senv. simpl.
-    unfold RelocProgSemantics.globalenv.
-    rewrite ! genv_senv_add_external_globals. simpl.
-    exploit strtable_encode_spec; eauto. exploit symbtable_encode_spec; eauto.
-    exploit reloctables_encode_spec; eauto. exploit shstrtable_encode_spec; eauto.
-    intuition congruence.
-  - intros s1 IS.
-    eexists; split; eauto.
-    econstructor.
-    unfold decode_tables.
-    rewrite shstr_decode. simpl.
-    rewrite reloc_decode. simpl.
-    rewrite symb_decode. simpl.
-    rewrite str_decode. simpl. eauto. apply IS.
-  - simpl. intuition congruence.
-  - simpl. intros.
-    rewrite genv_same. subst. eauto.
+  unfold semantics. rewrite decode_tables_correct.
+  eapply forward_simulation_step with (match_states := fun (e1 e2: Asm.state) => e1 = e2); simpl; intuition try congruence; subst; eauto.
 Qed.
 
 End PRESERVATION.
