x86/RelocElfgenproof.v
@@ -1,0 +1,139 @@
+(* *******************  *)
+(* Author: Pierre Wilke *)
+(* Date:   Jan 29, 2020 *)
+(* *******************  *)
+
+Require Import Coqlib Errors.
+Require Import Integers Floats AST Linking.
+Require Import Values Memory Events Globalenvs Smallstep.
+Require Import Op Locations Mach Conventions Asm RealAsm.
+Require Import RelocProgram RelocProgSemantics3.
+Require Import RelocElf RelocElfSemantics.
+Require Import RelocElfgen.
+Import ListNotations.
+
+Definition match_prog p tp :=
+  gen_reloc_elf p = OK tp.
+
+Lemma transf_program_match:
+  forall p tp, gen_reloc_elf p = OK tp -> match_prog p tp.
+Proof.
+  unfold match_prog; intuition.
+Qed.
+
+Section PRESERVATION.
+  Existing Instance inject_perm_all.
+Context `{external_calls_prf: ExternalCalls}.
+
+Local Existing Instance mem_accessors_default.
+
+
+Variable prog: RelocProgram.program.
+Variable tprog: elf_file.
+
+Hypothesis TRANSF: match_prog prog tprog.
+
+Hypothesis first_section_is_null:
+  hd_error (prog_sectable prog) = Some sec_null.
+
+Hypothesis decodable:
+  exists pp, decode_tables prog = OK pp.
+
+Lemma decode_tables_same:
+  decode_tables prog = decode_tables (reloc_program_of_elf_program tprog).
+Proof.
+  unfold match_prog in TRANSF. unfold gen_reloc_elf in TRANSF.
+  monadInv TRANSF. repeat destr_in EQ0.
+  unfold decode_tables.
+  unfold gen_sections in EQ. destr_in EQ.
+  assert (map sec_bytes x = s0).
+  {
+    revert EQ. clear. revert x.
+    induction s0; simpl; intros; eauto. inv EQ. reflexivity.
+    destruct (fold_right acc_sections (OK []) s0) eqn:?.
+    unfold acc_sections in EQ. simpl in EQ. monadInv EQ. simpl. f_equal.
+    unfold transl_section in EQ0. destr_in EQ0. eauto.
+    simpl in EQ. inv EQ.
+  }
+  unfold reloc_program_of_elf_program. simpl.
+  apply Nat.eqb_eq in Heqb.
+  destruct x; simpl in Heqb; try omega.
+  destruct x; simpl in Heqb; try omega.
+  destruct x; simpl in Heqb; try omega.
+  destruct x; simpl in Heqb; try omega.
+  destruct x; simpl in Heqb; try omega.
+  destruct x; simpl in Heqb; try omega.
+  destruct x; simpl in Heqb; try omega.
+  destruct x; simpl in Heqb; try omega.
+  simpl in first_section_is_null. inv first_section_is_null. subst. simpl.
+  auto.
+Qed.
+
+Lemma decode_tables_eq: forall p1 p2,
+    RelocProgram.prog_defs p1 = RelocProgram.prog_defs p2 ->
+    RelocProgram.prog_public p1 = RelocProgram.prog_public p2 ->
+    RelocProgram.prog_main p1 = RelocProgram.prog_main p2 ->
+    RelocProgram.prog_sectable p1 = RelocProgram.prog_sectable p2 ->
+    RelocProgram.prog_senv p1 = RelocProgram.prog_senv p2 ->
+    decode_tables p1 = decode_tables p2.
+Proof.
+  intros p1 p2 eq_defs eq_public eq_main eq_sectable eq_senv.
+  unfold decode_tables.
+  rewrite eq_sectable, eq_senv. unfold bind, bind2.
+  repeat (destr; [idtac]).  destr.
+Qed.
+
+Lemma semantics3same: forall p1 p2 rs,
+    RelocProgram.prog_defs p1 = RelocProgram.prog_defs p2 ->
+    RelocProgram.prog_public p1 = RelocProgram.prog_public p2 ->
+    RelocProgram.prog_main p1 = RelocProgram.prog_main p2 ->
+    RelocProgram.prog_sectable p1 = RelocProgram.prog_sectable p2 ->
+    RelocProgram.prog_senv p1 = RelocProgram.prog_senv p2 ->
+    (exists p, decode_tables p1 = OK p) ->
+    RelocProgSemantics3.semantics p1 rs = RelocProgSemantics3.semantics p2 rs.
+Proof.
+  intros p1 p2 rs eq_defs eq_public eq_main eq_sectable eq_senv (pp & DT).
+  unfold RelocProgSemantics3.semantics.
+  erewrite <- (decode_tables_eq p1 p2); eauto.
+  rewrite DT. auto.
+Qed.
+
+Lemma fr_acc_sections_map s0 x:
+  fold_right acc_sections (OK []) s0 = OK x -> s0 = sec_bytes ## x.
+Proof.
+  revert x; induction s0; simpl; intros; eauto. inv H; auto.
+  unfold acc_sections in H at 1. monadInv H. apply IHs0 in EQ. subst.
+  unfold transl_section in EQ1. destr_in EQ1. inv EQ1. auto.
+Qed.
+
+Lemma transf_program_correct:
+  forall rs, forward_simulation (RelocProgSemantics3.semantics prog rs)
+                                (RelocElfSemantics.semantics tprog rs).
+Proof.
+  unfold semantics. intro rs.
+  assert (EQ: RelocProgSemantics3.semantics prog rs =
+              RelocProgSemantics3.semantics (reloc_program_of_elf_program tprog) rs).
+  {
+    unfold match_prog, gen_reloc_elf in TRANSF.
+    monadInv TRANSF. repeat destr_in EQ0.
+    unfold reloc_program_of_elf_program. simpl.
+    apply semantics3same; simpl; auto.
+    destruct (prog_sectable prog); simpl in *; try congruence.
+    apply Nat.eqb_eq in Heqb.
+    destruct x; simpl in Heqb; try omega.
+    destruct x; simpl in Heqb; try omega.
+    destruct x; simpl in Heqb; try omega.
+    destruct x; simpl in Heqb; try omega.
+    destruct x; simpl in Heqb; try omega.
+    destruct x; simpl in Heqb; try omega.
+    destruct x; simpl in Heqb; try omega.
+    destruct x; simpl in Heqb; try omega.
+    inv first_section_is_null.
+    apply fr_acc_sections_map in EQ. subst. auto.
+  }
+  rewrite EQ.
+  eapply forward_simulation_step with (match_states := fun (e1 e2: Asm.state) => e1 = e2);
+    simpl; intros; subst; eauto.
+Qed.
+
+End PRESERVATION.
